

Homework #2 (due 02/08/26)

Instructor: Dr. Guanqun Cao (caoguanq@msu.edu)**Grader:** Andrews Boahen (boahenan@msu.edu)

All problems on this homework are from the required textbook [Applied Multivariate Statistical Analysis](#) (6th edition, by Johnson and Wichern).

Problems from Chapter 2

Problem 2.34*Solution*

Consider the vectors

$$\mathbf{b} = \begin{bmatrix} 2 \\ -1 \\ 4 \\ 0 \end{bmatrix}, \quad \mathbf{d} = \begin{bmatrix} -1 \\ 3 \\ -2 \\ 1 \end{bmatrix}.$$

The Cauchy-Schwarz inequality states that

$$(\mathbf{b}'\mathbf{d})^2 \leq (\mathbf{b}'\mathbf{b})(\mathbf{d}'\mathbf{d}).$$

We have:

$$\mathbf{b}'\mathbf{d} = -13,$$

$$\mathbf{b}'\mathbf{b} = 21 \quad \text{and}$$

$$\mathbf{d}'\mathbf{d} = 15.$$

Hence the inequality holds since,

$$(\mathbf{b}'\mathbf{d})^2 = 169 \quad \text{and} \quad (\mathbf{b}'\mathbf{b})(\mathbf{d}'\mathbf{d}) = 21 \times 15 = 315.$$

Problem 2.35*Solution*

Consider the vectors

$$\mathbf{b} = \begin{bmatrix} -4 \\ 3 \end{bmatrix}, \quad \mathbf{d} = \begin{bmatrix} 1 \\ 1 \end{bmatrix}$$

and the matrix

$$B = \begin{bmatrix} 2 & -2 \\ -2 & 5 \end{bmatrix}.$$

The extended Cauchy-Schwarz inequality states that

$$(\mathbf{b}'\mathbf{d})^2 \leq (\mathbf{b}'B\mathbf{b})(\mathbf{d}'B^{-1}\mathbf{d}).$$

We have:

$$\mathbf{b}'\mathbf{d} = -1,$$

$$\mathbf{b}'B\mathbf{b} = 125 \quad \text{and}$$

$$\mathbf{d}'B^{-1}\mathbf{d} = 11/6.$$

Therefore the inequality holds since,

$$(\mathbf{b}'\mathbf{d})^2 = 1 \quad \text{and} \quad (\mathbf{b}'B\mathbf{b})(\mathbf{d}'B^{-1}\mathbf{d}) = \frac{1375}{6}.$$

Problems from Chapter 3

Problem 3.14*Solution*

Consider the data matrix

$$X = \begin{bmatrix} 9 & 1 \\ 5 & 3 \\ 1 & 2 \end{bmatrix},$$

with $n = 3$ observations on $p = 2$ variables X_1 and X_2 . Form the linear combinations,

$$\mathbf{c}'\mathbf{X} = -X_1 + 2X_2, \quad \mathbf{b}'\mathbf{X} = 2X_1 + 3X_2.$$

the observed values are:

$$\begin{aligned} \mathbf{c}'\mathbf{X} : & \quad -7, 1, 3 \\ \mathbf{b}'\mathbf{X} : & \quad 21, 19, 8. \end{aligned}$$

a) From first principle, the respective sample means are then

$$\bar{c} = \frac{-7 + 1 + 3}{3} = -1, \quad \bar{b} = \frac{21 + 19 + 8}{3} = 16.$$

and sample variances are:

$$\begin{aligned} s_c &= \frac{(-7 + 1)^2 + (1 + 1)^2 + (3 + 1)^2}{2} = 28, \\ s_b &= \frac{(21 - 16)^2 + (19 - 16)^2 + (8 - 16)^2}{2} = 49. \end{aligned}$$

The sample covariance is then

$$s_{cb} = \frac{(-7 + 1)(21 - 16) + (1 + 1)(19 - 16) + (3 + 1)(8 - 16)}{2} = -28.$$

b) Using Formulas (3-36) and noting that the sample mean vector and covariance matrix are

$$\bar{\mathbf{x}} = \begin{bmatrix} 5 \\ 2 \end{bmatrix}, \quad S = \begin{bmatrix} 16 & -2 \\ -2 & 1 \end{bmatrix}$$

we get the means as:

$$\mathbf{c}'\bar{\mathbf{x}} = -1, \quad \mathbf{b}'\bar{\mathbf{x}} = 16,$$

and variances and covariance as:

$$\mathbf{c}'S\mathbf{c} = 28, \quad \mathbf{b}'S\mathbf{b} = 49, \quad \mathbf{c}'S\mathbf{b} = -28.$$

The results in (a) and (b) match.

Problem 3.16*Solution*

Proof. We have:

$$\begin{aligned} \Sigma &= \mathbf{E}[(\mathbf{V} - \boldsymbol{\mu})(\mathbf{V} - \boldsymbol{\mu})'] \\ &= \mathbf{E}(\mathbf{V}\mathbf{V}') - \mathbf{E}(\mathbf{V})\boldsymbol{\mu}' - \boldsymbol{\mu}\mathbf{E}(\mathbf{V}') + \boldsymbol{\mu}\boldsymbol{\mu}' \\ &= \mathbf{E}(\mathbf{V}\mathbf{V}') - \boldsymbol{\mu}\boldsymbol{\mu}' - \boldsymbol{\mu}\boldsymbol{\mu}' + \boldsymbol{\mu}\boldsymbol{\mu}' \\ &= \mathbf{E}(\mathbf{V}\mathbf{V}') - \boldsymbol{\mu}\boldsymbol{\mu}'. \end{aligned}$$

Rearranging gives the desired result:

$$\boxed{\mathbf{E}(\mathbf{V}\mathbf{V}') = \Sigma + \boldsymbol{\mu}\boldsymbol{\mu}'}.$$

□

Problems from Chapter 4

Problem 4.3*Solution*

Let $\mathbf{X} = (X_1, X_2, X_3)' \sim N_3(\boldsymbol{\mu}, \Sigma)$, where

$$\boldsymbol{\mu} = \begin{bmatrix} -3 \\ 1 \\ 4 \end{bmatrix}, \quad \Sigma = \begin{bmatrix} 1 & -2 & 0 \\ -2 & 5 & 0 \\ 0 & 0 & 2 \end{bmatrix}.$$

a) X_1 and X_2 are **not independent** since

$$\text{Cov}(X_1, X_2) = \Sigma_{12} = -2 \neq 0.$$

b) X_2 and X_3 are **independent** since X_2 and X_3 are jointly normal and

$$\text{Cov}(X_2, X_3) = \Sigma_{23} = 0.$$

c) $Y = (X_1, X_2)$ and X_3 are **independent** since

$$\text{Cov}(Y, X_3) = \Sigma_{Y, X_3} = (0, 0)'.$$

d) $\frac{X_1 + X_2}{2}$ and X_3 are **independent** since Y and X_3 are jointly normal and

$$\text{Cov}(X_1, X_3) = \text{Cov}(X_2, X_3) = 0.$$

e) X_2 and $Y = X_2 - \frac{5}{2}X_1 - X_3$ are **not independent** since

$$\text{Cov}(X_2, Y) = \text{Var}(X_2) - \frac{5}{2}\text{Cov}(X_1, X_2) = 10 \neq 0.$$

Problem 4.13*Solution*

Let $\mathbf{X} \sim N_p(\boldsymbol{\mu}, \Sigma)$ with $|\Sigma| \neq 0$. Partition \mathbf{X} , $\boldsymbol{\mu}$, and Σ conformably as

$$\mathbf{X} = \begin{bmatrix} \mathbf{X}_1 \\ \mathbf{X}_2 \end{bmatrix}, \quad \boldsymbol{\mu} = \begin{bmatrix} \boldsymbol{\mu}_1 \\ \boldsymbol{\mu}_2 \end{bmatrix}, \quad \Sigma = \begin{bmatrix} \Sigma_{11} & \Sigma_{12} \\ \Sigma_{21} & \Sigma_{22} \end{bmatrix},$$

where \mathbf{X}_1 is $q \times 1$, \mathbf{X}_2 is $(p - q) \times 1$, Σ_{22} is nonsingular, and $\Sigma_{21} = \Sigma'_{12}$.

a) *Proof.* Note that Σ can be decomposed as

$$\begin{aligned} \Sigma &= \begin{bmatrix} \Sigma_{11} & \Sigma_{12} \\ \Sigma_{21} & \Sigma_{22} \end{bmatrix} \\ &= \begin{bmatrix} \mathbf{I} & \Sigma_{12}\Sigma_{22}^{-1} \\ \mathbf{0} & \mathbf{I} \end{bmatrix} \begin{bmatrix} \Sigma_{11} - \Sigma_{12}\Sigma_{22}^{-1}\Sigma_{21} & \mathbf{0} \\ \Sigma_{21} & \Sigma_{22} \end{bmatrix} \\ &= \mathbf{AB} \end{aligned}$$

Using properties of determinant of block matrices, we get $|A| = |I| = 1$ and then

$$|\Sigma| = |\Sigma_{22}| |\Sigma_{11} - \Sigma_{12}\Sigma_{22}^{-1}\Sigma_{21}|$$

□

b) *Proof.* Using the hint from the textbook, we write

$$\begin{aligned} (\mathbf{x} - \boldsymbol{\mu})' \boldsymbol{\Sigma}^{-1} (\mathbf{x} - \boldsymbol{\mu}) &= \begin{bmatrix} \mathbf{x}_1 - \boldsymbol{\mu}_1 \\ \mathbf{x}_2 - \boldsymbol{\mu}_2 \end{bmatrix}' \begin{bmatrix} \mathbf{I} & \mathbf{0} \\ -\boldsymbol{\Sigma}_{22}^{-1} \boldsymbol{\Sigma}_{21} & \mathbf{I} \end{bmatrix} \begin{bmatrix} (\boldsymbol{\Sigma}_{11} - \boldsymbol{\Sigma}_{12}^{-1} \boldsymbol{\Sigma}_{22}^{-1} \boldsymbol{\Sigma}_{21})^{-1} & \mathbf{0} \\ \mathbf{0}' & \boldsymbol{\Sigma}_{22}^{-1} \end{bmatrix} \begin{bmatrix} \mathbf{I} & -\boldsymbol{\Sigma}_{12} \boldsymbol{\Sigma}_{22}^{-1} \\ \mathbf{0} & \mathbf{I} \end{bmatrix} \begin{bmatrix} \mathbf{x}_1 - \boldsymbol{\mu}_1 \\ \mathbf{x}_2 - \boldsymbol{\mu}_2 \end{bmatrix} \\ &= \begin{bmatrix} \mathbf{x}_1 - \boldsymbol{\mu}_1 \\ \mathbf{x}_2 - \boldsymbol{\mu}_2 \end{bmatrix}' \begin{bmatrix} \mathbf{I} & \mathbf{0} \\ -\boldsymbol{\Sigma}_{22}^{-1} \boldsymbol{\Sigma}_{21} & \mathbf{I} \end{bmatrix} \begin{bmatrix} (\boldsymbol{\Sigma}_{11} - \boldsymbol{\Sigma}_{12}^{-1} \boldsymbol{\Sigma}_{22}^{-1} \boldsymbol{\Sigma}_{21})^{-1} & \mathbf{0} \\ \mathbf{0}' & \boldsymbol{\Sigma}_{22}^{-1} \end{bmatrix} \begin{bmatrix} \mathbf{x}_1 - \boldsymbol{\mu}_1 - \boldsymbol{\Sigma}_{12} \boldsymbol{\Sigma}_{22}^{-1} (\mathbf{x}_2 - \boldsymbol{\mu}_2) \\ \mathbf{x}_2 - \boldsymbol{\mu}_2 \end{bmatrix} \end{aligned}$$

We arrive at the answer after the above matrix multiplication. \square

c) The result in b) shows that the quadratic form in the exponent of the multivariate normal density can be decomposed as

$$(\mathbf{x} - \boldsymbol{\mu})' \boldsymbol{\Sigma}^{-1} (\mathbf{x} - \boldsymbol{\mu}) = (\mathbf{x}_1 - \boldsymbol{\mu}_{1|2})' \boldsymbol{\Sigma}_{1|2}^{-1} (\mathbf{x}_1 - \boldsymbol{\mu}_{1|2}) + (\mathbf{x}_2 - \boldsymbol{\mu}_2)' \boldsymbol{\Sigma}_{22}^{-1} (\mathbf{x}_2 - \boldsymbol{\mu}_2),$$

where

$$\boldsymbol{\mu}_{1|2} = \boldsymbol{\mu}_1 + \boldsymbol{\Sigma}_{12} \boldsymbol{\Sigma}_{22}^{-1} (\mathbf{x}_2 - \boldsymbol{\mu}_2)$$

and

$$\boldsymbol{\Sigma}_{1|2} = \boldsymbol{\Sigma}_{11} - \boldsymbol{\Sigma}_{12} \boldsymbol{\Sigma}_{22}^{-1} \boldsymbol{\Sigma}_{21}$$

are the conditional mean and covariance of $\mathbf{X}_1 | \mathbf{X}_2 = \mathbf{x}_2$.

From parts (a) and (b), and the factorization of the multivariate normal density, we immediately obtain:

1. **Marginal distribution of \mathbf{X}_2 :**

$$\mathbf{X}_2 \sim N_{p-q}(\boldsymbol{\mu}_2, \boldsymbol{\Sigma}_{22}).$$

2. **Conditional distribution of**

$$\mathbf{X}_1 | \mathbf{X}_2 = \mathbf{x}_2 \sim N_q(\boldsymbol{\mu}_{1|2}, \boldsymbol{\Sigma}_{1|2}).$$

Problem 4.14

Solution

It follows from the previous problem that when $\boldsymbol{\Sigma}_{12} = 0$,

$$|\boldsymbol{\Sigma}| = |\boldsymbol{\Sigma}_{11}| |\boldsymbol{\Sigma}_{22}| \quad \text{and} \quad (\mathbf{x} - \boldsymbol{\mu})' \boldsymbol{\Sigma}^{-1} (\mathbf{x} - \boldsymbol{\mu}) = (\mathbf{x}_1 - \boldsymbol{\mu}_1)' \boldsymbol{\Sigma}_{11}^{-1} (\mathbf{x}_1 - \boldsymbol{\mu}_1) + (\mathbf{x}_2 - \boldsymbol{\mu}_2)' \boldsymbol{\Sigma}_{22}^{-1} (\mathbf{x}_2 - \boldsymbol{\mu}_2)$$

We can then easily rewrite the distribution of \mathbf{X} as a product of the marginals of \mathbf{X}_1 and \mathbf{X}_2 following the idea in the previous problem.

Problem 4.15

Solution

Proof. We have \mathbf{x}_j is a $p \times 1$ matrix and hence $\bar{\mathbf{x}}$ is $p \times 1$ and the product $(\mathbf{x}_j - \bar{\mathbf{x}})(\bar{\mathbf{x}} - \boldsymbol{\mu})'$ is a $p \times p$. Similarly, $(\bar{\mathbf{x}} - \boldsymbol{\mu})(\mathbf{x}_j - \bar{\mathbf{x}})'$ is $p \times p$. Now,

$$\sum_{i=1}^n (\mathbf{x}_j - \bar{\mathbf{x}})(\bar{\mathbf{x}} - \boldsymbol{\mu})' = n(\bar{\mathbf{x}} - \bar{\mathbf{x}})(\bar{\mathbf{x}} - \boldsymbol{\mu})' = 0$$

and

$$\sum_{i=1}^n (\bar{\mathbf{x}} - \boldsymbol{\mu})(\mathbf{x}_j - \bar{\mathbf{x}})' = (\bar{\mathbf{x}} - \boldsymbol{\mu})n(\bar{\mathbf{x}} - \bar{\mathbf{x}})' = 0$$

\square

Problem 4.16

Solution

a) **Marginal distributions for each of \mathbf{V}_1 and \mathbf{V}_2**

Both \mathbf{V}_1 and \mathbf{V}_2 are linear combinations of normal random variables and hence are normally distributed. Additionally, $\mathbf{X}_1, \dots, \mathbf{X}_4$ are independent. We then compute the first and second moments of both distributions.

$$\begin{aligned}\boldsymbol{\mu}_1 &= E[\mathbf{V}_1] = \frac{1}{4}E[\mathbf{X}_1] - \frac{1}{4}E[\mathbf{X}_2] + \frac{1}{4}E[\mathbf{X}_3] - \frac{1}{4}E[\mathbf{X}_4] = \mathbf{0}, \\ \boldsymbol{\Sigma}_1 &= \frac{1}{4}(4\boldsymbol{\Sigma}) = \boldsymbol{\Sigma}\end{aligned}$$

and

$$\begin{aligned}\boldsymbol{\mu}_2 &= E[\mathbf{V}_2] = \frac{1}{4}E[\mathbf{X}_1] + \frac{1}{4}E[\mathbf{X}_2] - \frac{1}{4}E[\mathbf{X}_3] - \frac{1}{4}E[\mathbf{X}_4] = \mathbf{0}, \\ \boldsymbol{\Sigma}_2 &= \frac{1}{4}(4\boldsymbol{\Sigma}) = \boldsymbol{\Sigma}\end{aligned}$$

b) **Joint distribution**

Note that

$$\begin{bmatrix} \mathbf{V}_1 \\ \mathbf{V}_2 \end{bmatrix} = \mathbf{A} \begin{bmatrix} \mathbf{X}_1 \\ \mathbf{X}_2 \\ \mathbf{X}_3 \\ \mathbf{X}_4 \end{bmatrix},$$

where $\mathbf{A} = \begin{bmatrix} \frac{1}{4} & -\frac{1}{4} & \frac{1}{4} & -\frac{1}{4} \\ \frac{1}{4} & \frac{1}{4} & -\frac{1}{4} & -\frac{1}{4} \end{bmatrix}$. We then have

$$\begin{bmatrix} \mathbf{V}_1 \\ \mathbf{V}_2 \end{bmatrix} \sim N_{2p}\left(\mathbf{A}\boldsymbol{\mu}, \mathbf{A}\boldsymbol{\Sigma}\mathbf{A}'\right) \equiv N_{2p}\left(\mathbf{0}, \mathbf{A}\boldsymbol{\Sigma}\mathbf{A}'\right)$$

Problem 4.19

Solution

- a) $(\mathbf{X}_1 - \boldsymbol{\mu})'\boldsymbol{\Sigma}^{-1}(\mathbf{X}_1 - \boldsymbol{\mu}) \sim \chi_6^2$
- b) $\bar{\mathbf{X}} \sim N_6\left(\boldsymbol{\mu}, \frac{\boldsymbol{\Sigma}}{20}\right)$ and $\sqrt{n}(\bar{\mathbf{X}} - \boldsymbol{\mu}) \sim N_6(0, \boldsymbol{\Sigma})$
- c) $19\mathbf{S} \sim W_6(19, \boldsymbol{\Sigma})$, where $W_6(19, \boldsymbol{\Sigma})$ is a Wishart distribution with 19 d.f.